Lists.v
@@ -1,31 +1,6 @@
 (** * Lists: Working with Structured Data *)
 
-(* $Date: 2012-09-08 14:51:57 -1000 (Sat, 08 Sep 2012) $ *)
-
-(** The next line imports all of our definitions from the
-    previous chapter. *)
 Require Export Induction.
-Require Export Basics.
-
-(** For it to work, you need to use [coqc] to compile [Basics.v]
-    into [Basics.vo].  (This is like making a .class file from a .java
-    file, or a .o file from a .c file.)
-  
-    Here are two ways to compile your code:
-  
-     - CoqIDE:
-   
-         Open [Basics.v].
-         In the "Compile" menu, click on "Compile Buffer".
-   
-     - Command line:
-   
-         Run [coqc Basics.v]
-
-    In this file, we again use the [Module] feature to wrap all of the
-    definitions for pairs and lists of numbers in a module so that,
-    later, we can reuse the same names for improved (generic) versions
-    of the same operations. *)
 
 Module NatList. 
 
@@ -33,7 +8,7 @@ Module NatList.
 (** * Pairs of Numbers *)
 
 (** In an [Inductive] type definition, each constructor can take
-    any number of parameters -- none (as with [true] and [O]), one (as
+    any number of arguments -- none (as with [true] and [O]), one (as
     with [S]), or more than one, as in this definition: *)
 
 Inductive natprod : Type :=
@@ -45,7 +20,9 @@ Inductive natprod : Type :=
 
 (** We can construct an element of [natprod] like this: *)
 
-Eval simpl in (pair 3 5).
+Check (pair 3 5).
+
+(** *** *)
 
 (** Here are two simple function definitions for extracting the
     first and second components of a pair.  (The definitions also
@@ -61,7 +38,10 @@ Definition snd (p : natprod) : nat :=
   | pair x y => y
   end.
 
-Eval simpl in (fst (pair 3 5)).
+Eval compute in (fst (pair 3 5)).
+(* ===> 3 *)
+
+(** *** *)
 
 (** Since pairs are used quite a bit, it is nice to be able to
     write them with the standard mathematical notation [(x,y)] instead
@@ -75,7 +55,7 @@ Notation "( x , y )" := (pair x y).
     chapter -- this notation is provided as part of the standard
     library): *)
 
-Eval simpl in (fst (3,5)).
+Eval compute in (fst (3,5)).
 
 Definition fst' (p : natprod) : nat := 
   match p with
@@ -91,6 +71,8 @@ Definition swap_pair (p : natprod) : natprod :=
   | (x,y) => (y,x)
   end.
 
+(** *** *)
+
 (** Let's try and prove a few simple facts about pairs.  If we
     state the lemmas in a particular (and slightly peculiar) way, we
     can prove them with just reflexivity (and its built-in
@@ -101,15 +83,16 @@ Theorem surjective_pairing' : forall (n m : nat),
 Proof.
   reflexivity.  Qed.
 
-(** But reflexivity is not enough if we state the lemma in a more
-    natural way: *)
+(** Note that [reflexivity] is not enough if we state the lemma in a
+    more natural way: *)
 
 Theorem surjective_pairing_stuck : forall (p : natprod),
   p = (fst p, snd p).
 Proof.
   simpl. (* Doesn't reduce anything! *)
-Admitted.
+Abort.
 
+(** *** *)
 (** We have to expose the structure of [p] so that [simpl] can
     perform the pattern match in [fst] and [snd].  We can do this with
     [destruct].
@@ -121,26 +104,21 @@ Admitted.
 Theorem surjective_pairing : forall (p : natprod),
   p = (fst p, snd p).
 Proof.
-  intros p.  destruct p as (n,m).  simpl.  reflexivity.  Qed.
+  intros p.  destruct p as [n m].  simpl.  reflexivity.  Qed.
 
-(** Notice that Coq allows us to use the notation we introduced
-    for pairs in the "[as]..." pattern that tells it what variables to
-    bind. *)
-
-(** **** Exercise: 1 star (snd_fst_is_swap) *)
+(** **** Exercise: 1 star (snd_fst_is_swap)  *)
 Theorem snd_fst_is_swap : forall (p : natprod),
   (snd p, fst p) = swap_pair p.
 Proof.
-  intros p. destruct p as (n, m).
-  simpl. reflexivity. Qed.
+  (* FILL IN HERE *) Admitted.
+(** [] *)
 
-
-(** **** Exercise: 1 star, optional (fst_swap_is_snd) *)
+(** **** Exercise: 1 star, optional (fst_swap_is_snd)  *)
 Theorem fst_swap_is_snd : forall (p : natprod),
   fst (swap_pair p) = snd p.
 Proof.
-  intros p. destruct p as (n, m).
-  simpl. reflexivity. Qed.
+  (* FILL IN HERE *) Admitted.
+(** [] *)
 
 (* ###################################################### *)
 (** * Lists of Numbers *)
@@ -158,6 +136,8 @@ Inductive natlist : Type :=
 
 Definition mylist := cons 1 (cons 2 (cons 3 nil)).
 
+
+(** *** *)
 (** As with pairs, it is more convenient to write lists in
     familiar programming notation.  The following two declarations
     allow us to use [::] as an infix [cons] operator and square
@@ -165,7 +145,7 @@ Definition mylist := cons 1 (cons 2 (cons 3 nil)).
 
 Notation "x :: l" := (cons x l) (at level 60, right associativity).
 Notation "[ ]" := nil.
-Notation "[ x , .. , y ]" := (cons x .. (cons y nil) ..).
+Notation "[ x ; .. ; y ]" := (cons x .. (cons y nil) ..).
 
 (** It is not necessary to fully understand these declarations,
     but in case you are interested, here is roughly what's going on.
@@ -176,7 +156,7 @@ Notation "[ x , .. , y ]" := (cons x .. (cons y nil) ..).
 
 Definition mylist1 := 1 :: (2 :: (3 :: nil)).
 Definition mylist2 := 1 :: 2 :: 3 :: nil.
-Definition mylist3 := [1,2,3].
+Definition mylist3 := [1;2;3].
 
 (** The [at level 60] part tells Coq how to parenthesize
     expressions that involve both [::] and some other infix operator.
@@ -191,9 +171,9 @@ Notation "x + y" := (plus x y)
    (By the way, it's worth noting in passing that expressions like "[1
    + 2 :: [3]]" can be a little confusing when you read them in a .v
    file.  The inner brackets, around 3, indicate a list, but the outer
-   brackets are there to instruct the "coqdoc" tool that the bracketed
-   part should be displayed as Coq code rather than running text.
-   These brackets don't appear in the generated HTML.)
+   brackets, which are invisible in the HTML rendering, are there to
+   instruct the "coqdoc" tool that the bracketed part should be
+   displayed as Coq code rather than running text.)
 
    The second and third [Notation] declarations above introduce the
    standard square-bracket notation for lists; the right-hand side of
@@ -201,6 +181,7 @@ Notation "x + y" := (plus x y)
    notations and translating them to nested sequences of binary
    constructors. *)
 
+(** *** Repeat *)
 (** A number of functions are useful for manipulating lists.
     For example, the [repeat] function takes a number [n] and a
     [count] and returns a list of length [count] where every element
@@ -212,6 +193,7 @@ Fixpoint repeat (n count : nat) : natlist :=
   | S count' => n :: (repeat n count')
   end.
 
+(** *** Length *)
 (** The [length] function calculates the length of a list. *)
 
 Fixpoint length (l:natlist) : nat := 
@@ -220,6 +202,7 @@ Fixpoint length (l:natlist) : nat :=
   | h :: t => S (length t)
   end.
 
+(** *** Append *)
 (** The [app] ("append") function concatenates two lists. *)
 
 Fixpoint app (l1 l2 : natlist) : natlist := 
@@ -234,95 +217,69 @@ Fixpoint app (l1 l2 : natlist) : natlist :=
 Notation "x ++ y" := (app x y) 
                      (right associativity, at level 60).
 
-Example test_app1:             [1,2,3] ++ [4,5] = [1,2,3,4,5].
+Example test_app1:             [1;2;3] ++ [4;5] = [1;2;3;4;5].
 Proof. reflexivity.  Qed.
-Example test_app2:             nil ++ [4,5] = [4,5].
+Example test_app2:             nil ++ [4;5] = [4;5].
 Proof. reflexivity.  Qed.
-Example test_app3:             [1,2,3] ++ nil = [1,2,3].
+Example test_app3:             [1;2;3] ++ nil = [1;2;3].
 Proof. reflexivity.  Qed.
 
 (** Here are two smaller examples of programming with lists.
     The [hd] function returns the first element (the "head") of the
-    list, while [tail] returns everything but the first
-    element.  Of course, the empty list has no first element, so we
+    list, while [tl] returns everything but the first
+    element (the "tail").  
+    Of course, the empty list has no first element, so we
     must pass a default value to be returned in that case.  *)
 
+(** *** Head (with default) and Tail *)
 Definition hd (default:nat) (l:natlist) : nat :=
   match l with
   | nil => default
   | h :: t => h
   end.
 
-Definition tail (l:natlist) : natlist :=
+Definition tl (l:natlist) : natlist :=
   match l with
   | nil => nil  
   | h :: t => t
   end.
 
-Example test_hd1:             hd 0 [1,2,3] = 1.
+Example test_hd1:             hd 0 [1;2;3] = 1.
 Proof. reflexivity.  Qed.
 Example test_hd2:             hd 0 [] = 0.
 Proof. reflexivity.  Qed.
-Example test_tail:            tail [1,2,3] = [2,3].
+Example test_tl:              tl [1;2;3] = [2;3].
 Proof. reflexivity.  Qed.
 
-(** **** Exercise: 2 stars, recommended (list_funs) *)
+(** **** Exercise: 2 stars (list_funs)  *)
 (** Complete the definitions of [nonzeros], [oddmembers] and
-    [countoddmembers] below.  *)
+    [countoddmembers] below. Have a look at the tests to understand
+    what these functions should do. *)
 
 Fixpoint nonzeros (l:natlist) : natlist :=
-  match l with
-    | nil => nil
-    | h :: t => match h with
-                  | O => nonzeros t
-                  | S h' => h :: nonzeros t
-                end
-  end.
+  (* FILL IN HERE *) admit.
 
-
-Example test_nonzeros:            nonzeros [0,1,0,2,3,0,0] = [1,2,3].
-Proof. simpl. reflexivity. Qed.
-
-Fixpoint oddb (n:nat) : bool :=
-  match n with
-    | O        => false
-    | S O      => true
-    | S (S n') => oddb n'
-  end.
+Example test_nonzeros:            nonzeros [0;1;0;2;3;0;0] = [1;2;3].
+ (* FILL IN HERE *) Admitted.
 
 Fixpoint oddmembers (l:natlist) : natlist :=
-  match l with
-    | nil => nil
-    | h :: t => match oddb h with
-                  | true => h :: oddmembers t
-                  | false => oddmembers t
-                end
-  end.
+  (* FILL IN HERE *) admit.
 
-
-Example test_oddmembers:            oddmembers [0,1,0,2,3,0,0] = [1,3].
-Proof. simpl. reflexivity. Qed.
-
+Example test_oddmembers:            oddmembers [0;1;0;2;3;0;0] = [1;3].
+ (* FILL IN HERE *) Admitted.
 
 Fixpoint countoddmembers (l:natlist) : nat :=
-  match l with
-    | nil => O
-    | h :: t => match oddb h with
-                  | true => S (countoddmembers t)
-                  | false => countoddmembers t
-                end
-  end.
+  (* FILL IN HERE *) admit.
 
-Example test_countoddmembers1:    countoddmembers [1,0,3,1,4,5] = 4.
-Proof. simpl. reflexivity. Qed.
-
-Example test_countoddmembers2:    countoddmembers [0,2,4] = 0.
-Proof. simpl. reflexivity. Qed.
-
+Example test_countoddmembers1:    countoddmembers [1;0;3;1;4;5] = 4.
+ (* FILL IN HERE *) Admitted.
+Example test_countoddmembers2:    countoddmembers [0;2;4] = 0.
+ (* FILL IN HERE *) Admitted.
 Example test_countoddmembers3:    countoddmembers nil = 0.
-Proof. simpl. reflexivity. Qed.
+ (* FILL IN HERE *) Admitted.
+(** [] *)
 
-(** **** Exercise: 3 stars, recommended (alternate) *)
+(** **** Exercise: 3 stars, advanced (alternate)  *)
 (** Complete the definition of [alternate], which "zips up" two lists
     into one, alternating between elements taken from the first list
     and elements from the second.  See the tests below for more
@@ -337,26 +294,17 @@ Proof. simpl. reflexivity. Qed.
 
 
 Fixpoint alternate (l1 l2 : natlist) : natlist :=
-  match l1 with
-    | nil => l2
-    | a :: l1' => match l2 with
-                    | nil => l1
-                    | b :: l2' => a :: b :: alternate l1' l2'
-                  end
-  end.
+  (* FILL IN HERE *) admit.
 
 
-Example test_alternate1:        alternate [1,2,3] [4,5,6] = [1,4,2,5,3,6].
-Proof. simpl. reflexivity. Qed.
-
-Example test_alternate2:        alternate [1] [4,5,6] = [1,4,5,6].
-Proof. simpl. reflexivity. Qed.
-
-Example test_alternate3:        alternate [1,2,3] [4] = [1,4,2,3].
-Proof. simpl. reflexivity. Qed.
-
-Example test_alternate4:        alternate [] [20,30] = [20,30].
-Proof. simpl. reflexivity. Qed.
+Example test_alternate1:        alternate [1;2;3] [4;5;6] = [1;4;2;5;3;6].
+ (* FILL IN HERE *) Admitted.
+Example test_alternate2:        alternate [1] [4;5;6] = [1;4;5;6].
+ (* FILL IN HERE *) Admitted.
+Example test_alternate3:        alternate [1;2;3] [4] = [1;4;2;3].
+ (* FILL IN HERE *) Admitted.
+Example test_alternate4:        alternate [] [20;30] = [20;30].
+ (* FILL IN HERE *) Admitted. 
 (** [] *)
 
 (* ###################################################### *)
@@ -369,27 +317,19 @@ Proof. simpl. reflexivity. Qed.
 
 Definition bag := natlist.  
 
-(** **** Exercise: 3 stars, recommended (bag_functions) *)
+(** **** Exercise: 3 stars (bag_functions)  *)
 (** Complete the following definitions for the functions
     [count], [sum], [add], and [member] for bags. *)
 
-
 Fixpoint count (v:nat) (s:bag) : nat := 
-  match s with
-    | nil => O
-    | a :: s' => match beq_nat a v with
-                   | true => S (count v s')
-                   | false => count v s'
-                 end
-  end.
-
+  (* FILL IN HERE *) admit.
 
 (** All these proofs can be done just by [reflexivity]. *)
 
-Example test_count1:              count 1 [1,2,3,1,4,1] = 3.
-Proof. simpl. reflexivity. Qed.
-Example test_count2:              count 6 [1,2,3,1,4,1] = 0.
-Proof. reflexivity. Qed.
+Example test_count1:              count 1 [1;2;3;1;4;1] = 3.
+ (* FILL IN HERE *) Admitted.
+Example test_count2:              count 6 [1;2;3;1;4;1] = 0.
+ (* FILL IN HERE *) Admitted.
 
 (** Multiset [sum] is similar to set [union]: [sum a b] contains
     all the elements of [a] and of [b].  (Mathematicians usually
@@ -403,117 +343,70 @@ Proof. reflexivity. Qed.
     think about whether [sum] can be implemented in another way --
     perhaps by using functions that have already been defined.  *)
 
-Definition sum : bag -> bag -> bag :=
-  app.
-  
-  
-Example test_sum1:              count 1 (sum [1,2,3] [1,4,1]) = 3.
-Proof. simpl. reflexivity. Qed.
+Definition sum : bag -> bag -> bag := 
+  (* FILL IN HERE *) admit.
 
+Example test_sum1:              count 1 (sum [1;2;3] [1;4;1]) = 3.
+ (* FILL IN HERE *) Admitted.
 
-Definition add (v:nat) (s:bag) : bag :=
-  v :: s.
+Definition add (v:nat) (s:bag) : bag := 
+  (* FILL IN HERE *) admit.
 
-
-Example test_add1:                count 1 (add 1 [1,4,1]) = 3.
-Proof. simpl. reflexivity. Qed.
-
-Example test_add2:                count 5 (add 1 [1,4,1]) = 0.
-Proof. simpl. reflexivity. Qed.
+Example test_add1:                count 1 (add 1 [1;4;1]) = 3.
+ (* FILL IN HERE *) Admitted.
+Example test_add2:                count 5 (add 1 [1;4;1]) = 0.
+ (* FILL IN HERE *) Admitted.
 
 Definition member (v:nat) (s:bag) : bool := 
-  match count v s with
-    | O => false
-    | S a => true
-  end.
+  (* FILL IN HERE *) admit.
 
-Example test_member1:             member 1 [1,4,1] = true.
-Proof. reflexivity. Qed.
-Example test_member2:             member 2 [1,4,1] = false.
-Proof. reflexivity. Qed.
+Example test_member1:             member 1 [1;4;1] = true.
+ (* FILL IN HERE *) Admitted.
+Example test_member2:             member 2 [1;4;1] = false.
+ (* FILL IN HERE *) Admitted.
 (** [] *)
 
-(** **** Exercise: 3 stars, optional (bag_more_functions) *)
+(** **** Exercise: 3 stars, optional (bag_more_functions)  *)
 (** Here are some more bag functions for you to practice with. *)
 
 Fixpoint remove_one (v:nat) (s:bag) : bag :=
-  match s with
-    | nil => nil
-    | a :: s' => match beq_nat v a with
-                   | false => a :: remove_one v s'
-                   | true => s'
-                 end
-  end.
+  (* When remove_one is applied to a bag without the number to remove,
+     it should return the same bag unchanged. *)
+  (* FILL IN HERE *) admit.
 
-
-Example test_remove_one1:         count 5 (remove_one 5 [2,1,5,4,1]) = 0.
-Proof. simpl. reflexivity. Qed.
-
-Example test_remove_one2:         count 5 (remove_one 5 [2,1,4,1]) = 0.
-Proof. simpl. reflexivity. Qed.
-
-Example test_remove_one3:         count 4 (remove_one 5 [2,1,4,5,1,4]) = 2.
-Proof. simpl. reflexivity. Qed.
-
-Example test_remove_one4: 
-  count 5 (remove_one 5 [2,1,5,4,5,1,4]) = 1.
-Proof. simpl. reflexivity. Qed.
-
+Example test_remove_one1:         count 5 (remove_one 5 [2;1;5;4;1]) = 0.
+ (* FILL IN HERE *) Admitted.
+Example test_remove_one2:         count 5 (remove_one 5 [2;1;4;1]) = 0.
+ (* FILL IN HERE *) Admitted.
+Example test_remove_one3:         count 4 (remove_one 5 [2;1;4;5;1;4]) = 2.
+ (* FILL IN HERE *) Admitted.
+Example test_remove_one4:         count 5 (remove_one 5 [2;1;5;4;5;1;4]) = 1.
+ (* FILL IN HERE *) Admitted.
 
 Fixpoint remove_all (v:nat) (s:bag) : bag :=
-   match s with
-    | nil => nil
-    | a :: s' => match beq_nat v a with
-                   | false => a :: remove_all v s'
-                   | true => remove_all v s'
-                 end
-  end.
+  (* FILL IN HERE *) admit.
 
-
-Example test_remove_all1:          count 5 (remove_all 5 [2,1,5,4,1]) = 0.
-Proof. simpl. reflexivity. Qed.
-
-Example test_remove_all2:          count 5 (remove_all 5 [2,1,4,1]) = 0.
-Proof. simpl. reflexivity. Qed.
-
-Example test_remove_all3:          count 4 (remove_all 5 [2,1,4,5,1,4]) = 2.
-Proof. simpl. reflexivity. Qed.
-
-Example test_remove_all4:          count 5 (remove_all 5 [2,1,5,4,5,1,4,5,1,4]) = 0.
-Proof. simpl. reflexivity. Qed.
-
-Fixpoint equ (s1: bag) (s2 : bag) : bool :=
-  match s1 with
-    | nil => true
-    | a :: s1' => match s2 with
-                    | nil => false
-                    | b :: s2' => match beq_nat a b with
-                                    | false => false
-                                    | true => equ s1' s2'
-                                  end
-                  end
-  end.
+Example test_remove_all1:          count 5 (remove_all 5 [2;1;5;4;1]) = 0.
+ (* FILL IN HERE *) Admitted.
+Example test_remove_all2:          count 5 (remove_all 5 [2;1;4;1]) = 0.
+ (* FILL IN HERE *) Admitted.
+Example test_remove_all3:          count 4 (remove_all 5 [2;1;4;5;1;4]) = 2.
+ (* FILL IN HERE *) Admitted.
+Example test_remove_all4:          count 5 (remove_all 5 [2;1;5;4;5;1;4;5;1;4]) = 0.
+ (* FILL IN HERE *) Admitted.
 
 Fixpoint subset (s1:bag) (s2:bag) : bool :=
-  match s1 with
-    | nil => true
-    | a :: s1' => match equ s2 (remove_one a s2) with
-                    | true => false
-                    | false => subset s1' (remove_one a s2)
-                  end
-  end.
+  (* FILL IN HERE *) admit.
 
-
-Example test_subset1:              subset [1,2] [2,1,4,1] = true.
-Proof. simpl. reflexivity. Qed.
-
-Example test_subset2:              subset [1,2,2] [2,1,4,1] = false.
-Proof. simpl. reflexivity. Qed.
+Example test_subset1:              subset [1;2] [2;1;4;1] = true.
+ (* FILL IN HERE *) Admitted.
+Example test_subset2:              subset [1;2;2] [2;1;4;1] = false.
+ (* FILL IN HERE *) Admitted.
 (** [] *)
 
-(** **** Exercise: 3 stars, recommended (bag_theorem) *)
-(** Write down an interesting theorem about bags involving the
-    functions [count] and [add], and prove it.  Note that, since this
+(** **** Exercise: 3 stars (bag_theorem)  *)
+(** Write down an interesting theorem [bag_theorem] about bags involving
+    the functions [count] and [add], and prove it.  Note that, since this
     problem is somewhat open-ended, it's possible that you may come up
     with a theorem which is true, but whose proof requires techniques
     you haven't learned yet.  Feel free to ask for help if you get
@@ -532,8 +425,7 @@ Proof. simpl. reflexivity. Qed.
 
 Theorem nil_app : forall l:natlist,
   [] ++ l = l.
-Proof.
-   reflexivity.  Qed.
+Proof. reflexivity. Qed.
 
 (** ... because the [[]] is substituted into the match position
     in the definition of [app], allowing the match itself to be
@@ -543,9 +435,8 @@ Proof.
     analysis on the possible shapes (empty or non-empty) of an unknown
     list. *)
 
-
 Theorem tl_length_pred : forall l:natlist,
-  pred (length l) = length (tail l).
+  pred (length l) = length (tl l).
 Proof.
   intros l. destruct l as [| n l'].
   Case "l = nil".
@@ -554,7 +445,7 @@ Proof.
     reflexivity.  Qed.
 
 (** Here, the [nil] case works because we've chosen to define
-    [tail nil = nil]. Notice that the [as] annotation on the [destruct]
+    [tl nil = nil]. Notice that the [as] annotation on the [destruct]
     tactic here introduces two names, [n] and [l'], corresponding to
     the fact that the [cons] constructor for lists takes two
     arguments (the head and tail of the list it is constructing). *)
@@ -565,11 +456,11 @@ Proof.
 (* ###################################################### *)
 (** ** Micro-Sermon *)
 
-(** Simply reading example proofs will not get you very far!  It is
-    very important to work through the details of each one, using Coq
-    and thinking about what each step of the proof achieves.
-    Otherwise it is more or less guaranteed that the exercises will
-    make no sense. *)
+(** Simply reading example proof scripts will not get you very far!
+    It is very important to work through the details of each one,
+    using Coq and thinking about what each step achieves.  Otherwise
+    it is more or less guaranteed that the exercises will make no
+    sense... *)
 
 (* ###################################################### *)
 (** ** Induction on Lists *)
@@ -602,7 +493,7 @@ Proof.
     eventually reaching [nil], these two things together establish the
     truth of [P] for all lists [l].  Here's a concrete example: *)
 
-Theorem app_ass : forall l1 l2 l3 : natlist, 
+Theorem app_assoc : forall l1 l2 l3 : natlist, 
   (l1 ++ l2) ++ l3 = l1 ++ (l2 ++ l3).   
 Proof.
   intros l1 l2 l3. induction l1 as [| n l1'].
@@ -621,6 +512,8 @@ Proof.
     help the reader stay oriented if we remind them exactly what the
     induction hypothesis is in the second case.  *)
 
+(** *** Informal version *)
+
 (** _Theorem_: For all lists [l1], [l2], and [l3], 
    [(l1 ++ l2) ++ l3 = l1 ++ (l2 ++ l3)].
 
@@ -638,8 +531,11 @@ Proof.
      By the definition of [++], this follows from
        n :: ((l1' ++ l2) ++ l3) = n :: (l1' ++ (l2 ++ l3)),
      which is immediate from the induction hypothesis.  []
+*)
 
-  Here is an exercise to be worked together in class: *)
+(** *** Another example *)
+(**
+  Here is a similar example to be worked together in class: *)
 
 Theorem app_length : forall l1 l2 : natlist, 
   length (l1 ++ l2) = (length l1) + (length l2).
@@ -651,6 +547,8 @@ Proof.
   Case "l1 = cons".
     simpl. rewrite -> IHl1'. reflexivity.  Qed.
 
+
+(** *** Reversing a list *)
 (** For a slightly more involved example of an inductive proof
     over lists, suppose we define a "cons on the right" function
     [snoc] like this... *)
@@ -670,11 +568,12 @@ Fixpoint rev (l:natlist) : natlist :=
   | h :: t => snoc (rev t) h
   end.
 
-Example test_rev1:            rev [1,2,3] = [3,2,1].
+Example test_rev1:            rev [1;2;3] = [3;2;1].
 Proof. reflexivity.  Qed.
 Example test_rev2:            rev nil = nil.
 Proof. reflexivity.  Qed.
 
+(** *** Proofs about reverse *)
 (** Now let's prove some more list theorems using our newly
     defined [snoc] and [rev].  For something a little more challenging
     than the inductive proofs we've seen so far, let's prove that
@@ -688,21 +587,23 @@ Proof.
   Case "l = []".
     reflexivity.
   Case "l = n :: l'".
-    (* This is the tricky case.  Let's begin as usual by simplifying. *)
+    (* This is the tricky case.  Let's begin as usual 
+       by simplifying. *)
     simpl. 
-    (* Now we seem to be stuck: the goal is an equality involving
-       [snoc], but we don't have any equations in either the
-       immediate context or the global environment that have
-       anything to do with [snoc]! 
+    (* Now we seem to be stuck: the goal is an equality 
+       involving [snoc], but we don't have any equations 
+       in either the immediate context or the global 
+       environment that have anything to do with [snoc]! 
 
-       We can make a little progress by using the IH to rewrite the 
-       goal... *)
+       We can make a little progress by using the IH to 
+       rewrite the goal... *)
     rewrite <- IHl'.
     (* ... but now we can't go any further. *)
-Admitted.
+Abort.
 
 (** So let's take the equation about [snoc] that would have
-    enabled us to make progress and prove it as a separate lemma. *)
+    enabled us to make progress and prove it as a separate lemma. 
+*)
 
 Theorem length_snoc : forall n : nat, forall l : natlist,
   length (snoc l n) = S (length l).
@@ -713,6 +614,15 @@ Proof.
   Case "l = cons n' l'".
     simpl. rewrite -> IHl'. reflexivity.  Qed. 
 
+(**
+    Note that we make the lemma as _general_ as possible: in particular,
+    we quantify over _all_ [natlist]s, not just those that result
+    from an application of [rev]. This should seem natural, 
+    because the truth of the goal clearly doesn't depend on 
+    the list having been reversed.  Moreover, it is much easier
+    to prove the more general property. 
+*)
+    
 (** Now we can complete the original proof. *)
 
 Theorem rev_length : forall l : natlist,
@@ -768,10 +678,10 @@ Proof.
 
 (** Obviously, the style of these proofs is rather longwinded
     and pedantic.  After the first few, we might find it easier to
-    follow proofs that give a little less detail overall (since we can
-    easily work them out in our own minds or on scratch paper if
-    necessary) and just highlight the non-obvious steps.  In this more
-    compressed style, the above proof might look more like this: *)
+    follow proofs that give fewer details (since we can easily work
+    them out in our own minds or on scratch paper if necessary) and
+    just highlight the non-obvious steps.  In this more compressed
+    style, the above proof might look more like this: *)
 
 (** _Theorem_:
      For all lists [l], [length (rev l) = length l].
@@ -805,11 +715,11 @@ Proof.
     involving [foo].  For example, try uncommenting the following to
     see a list of theorems that we have proved about [rev]: *)
 
-(* SearchAbout rev. *)
+(*  SearchAbout rev. *)
 
 (** Keep [SearchAbout] in mind as you do the following exercises and
     throughout the rest of the course; it can save you a lot of time! *)
-    
+
 (** Also, if you are using ProofGeneral, you can run [SearchAbout]
     with [C-c C-a C-a]. Pasting its response into your buffer can be
     accomplished with [C-c C-;]. *)
@@ -817,7 +727,7 @@ Proof.
 (* ###################################################### *)
 (** ** List Exercises, Part 1 *)
 
-(** **** Exercise: 3 stars, recommended (list_exercises) *)
+(** **** Exercise: 3 stars (list_exercises)  *)
 (** More practice with lists. *)
 
 Theorem app_nil_end : forall l : natlist, 
@@ -835,7 +745,7 @@ Proof.
     yourself getting tangled up, step back and try to look for a
     simpler way. *)
 
-Theorem app_ass4 : forall l1 l2 l3 l4 : natlist,
+Theorem app_assoc4 : forall l1 l2 l3 l4 : natlist,
   l1 ++ (l2 ++ (l3 ++ l4)) = ((l1 ++ l2) ++ l3) ++ l4.
 Proof.
   (* FILL IN HERE *) Admitted.
@@ -853,8 +763,29 @@ Proof.
 
 (** An exercise about your implementation of [nonzeros]: *)
 
-Lemma nonzeros_length : forall l1 l2 : natlist,
+Lemma nonzeros_app : forall l1 l2 : natlist,
   nonzeros (l1 ++ l2) = (nonzeros l1) ++ (nonzeros l2).
+Proof.
+  (* FILL IN HERE *) Admitted.
+(** [] *)
+
+(** **** Exercise: 2 stars (beq_natlist)  *)
+(** Fill in the definition of [beq_natlist], which compares
+    lists of numbers for equality.  Prove that [beq_natlist l l]
+    yields [true] for every list [l]. *)
+
+Fixpoint beq_natlist (l1 l2 : natlist) : bool :=
+  (* FILL IN HERE *) admit.
+
+Example test_beq_natlist1 :   (beq_natlist nil nil = true).
+ (* FILL IN HERE *) Admitted.
+Example test_beq_natlist2 :   beq_natlist [1;2;3] [1;2;3] = true.
+ (* FILL IN HERE *) Admitted.
+Example test_beq_natlist3 :   beq_natlist [1;2;3] [1;2;4] = false.
+ (* FILL IN HERE *) Admitted.
+
+Theorem beq_natlist_refl : forall l:natlist,
+  true = beq_natlist l l.
 Proof.
   (* FILL IN HERE *) Admitted.
 (** [] *)
@@ -862,26 +793,23 @@ Proof.
 (* ###################################################### *)
 (** ** List Exercises, Part 2 *)
 
-(** **** Exercise: 2 stars, recommended (list_design) *)
+(** **** Exercise: 2 stars (list_design)  *)
 (** Design exercise: 
-     - Write down a non-trivial theorem involving [cons]
-       ([::]), [snoc], and [append] ([++]).  
+     - Write down a non-trivial theorem [cons_snoc_app]
+       involving [cons] ([::]), [snoc], and [app] ([++]).  
      - Prove it. *) 
 
 (* FILL IN HERE *)
 (** [] *)
 
-(** **** Exercise: 2 stars, optional (bag_proofs) *)
-(** If you did the optional exercise about bags above, here are a
-    couple of little theorems to prove about your definitions. *)
+(** **** Exercise: 3 stars, advanced (bag_proofs)  *)
+(** Here are a couple of little theorems to prove about your
+    definitions about bags earlier in the file. *)
 
 Theorem count_member_nonzero : forall (s : bag),
   ble_nat 1 (count 1 (1 :: s)) = true.
 Proof.
-  intros.
-  simpl.
-  reflexivity.
-  Qed.
+  (* FILL IN HERE *) Admitted.
 
 (** The following lemma about [ble_nat] might help you in the next proof. *)
 
@@ -900,14 +828,14 @@ Proof.
   (* FILL IN HERE *) Admitted.
 (** [] *)
 
-(** **** Exercise: 3 stars, optional (bag_count_sum) *)  
-(** Write down an interesting theorem about bags involving the
-    functions [count] and [sum], and prove it.*)
+(** **** Exercise: 3 stars, optional (bag_count_sum)  *)  
+(** Write down an interesting theorem [bag_count_sum] about bags 
+    involving the functions [count] and [sum], and prove it.*)
 
 (* FILL IN HERE *)
 (** [] *)
 
-(** **** Exercise: 4 stars, optional (rev_injective) *)
+(** **** Exercise: 4 stars, advanced (rev_injective)  *)
 (** Prove that the [rev] function is injective, that is,
 
     forall (l1 l2 : natlist), rev l1 = rev l2 -> l1 = l2.
@@ -922,12 +850,6 @@ There is a hard way and an easy way to solve this exercise.
 (* ###################################################### *)
 (** * Options *)
 
-(** Here is another type definition that is often useful in
-    day-to-day programming: *)
-
-Inductive natoption : Type :=
-  | Some : nat -> natoption
-  | None : natoption.  
 
 (** One use of [natoption] is as a way of returning "error
     codes" from functions.  For example, suppose we want to write a
@@ -944,10 +866,16 @@ Fixpoint index_bad (n:nat) (l:natlist) : nat :=
                end
   end.
 
+(** *** *)
 (** On the other hand, if we give it type [nat -> natlist ->
     natoption], then we can return [None] when the list is too short
     and [Some a] when the list has enough members and [a] appears at
     position [n]. *)
+
+Inductive natoption : Type :=
+  | Some : nat -> natoption
+  | None : natoption.  
+
 
 Fixpoint index (n:nat) (l:natlist) : natoption :=
   match l with
@@ -958,16 +886,18 @@ Fixpoint index (n:nat) (l:natlist) : natoption :=
                end
   end.
 
-Example test_index1 :    index 0 [4,5,6,7]  = Some 4.
+Example test_index1 :    index 0 [4;5;6;7]  = Some 4.
 Proof. reflexivity.  Qed.
-Example test_index2 :    index 3 [4,5,6,7]  = Some 7.
+Example test_index2 :    index 3 [4;5;6;7]  = Some 7.
 Proof. reflexivity.  Qed.
-Example test_index3 :    index 10 [4,5,6,7] = None.
+Example test_index3 :    index 10 [4;5;6;7] = None.
 Proof. reflexivity.  Qed.
 
 (** This example is also an opportunity to introduce one more
     small feature of Coq's programming language: conditional
     expressions... *)
+
+(** *** *)
 
 Fixpoint index' (n:nat) (l:natlist) : natoption :=
   match l with
@@ -992,92 +922,34 @@ Definition option_elim (d : nat) (o : natoption) : nat :=
   | None => d
   end.
 
-(** **** Exercise: 2 stars (hd_opt) *)
+(** **** Exercise: 2 stars (hd_opt)  *)
 (** Using the same idea, fix the [hd] function from earlier so we don't
    have to pass a default element for the [nil] case.  *)
 
 Definition hd_opt (l : natlist) : natoption :=
-  match l with
-    | nil => None
-    | a :: l' => Some a
-  end.
- 
+  (* FILL IN HERE *) admit.
 
 Example test_hd_opt1 : hd_opt [] = None.
-Proof. simpl. reflexivity. Qed.
-
+ (* FILL IN HERE *) Admitted.
 
 Example test_hd_opt2 : hd_opt [1] = Some 1.
-Proof. reflexivity. Qed.
+ (* FILL IN HERE *) Admitted.
 
-Example test_hd_opt3 : hd_opt [5,6] = Some 5.
-Proof. reflexivity. Qed.
+Example test_hd_opt3 : hd_opt [5;6] = Some 5.
+ (* FILL IN HERE *) Admitted.
 (** [] *)
 
-(** **** Exercise: 1 star, optional (option_elim_hd) *)
+(** **** Exercise: 1 star, optional (option_elim_hd)  *)
 (** This exercise relates your new [hd_opt] to the old [hd]. *)
 
 Theorem option_elim_hd : forall (l:natlist) (default:nat),
   hd default l = option_elim default (hd_opt l).
 Proof.
-  intros. induction l as [| l'].
-  Case "[]".
-  simpl. reflexivity.
-  Case "not []".
-  simpl.
-  reflexivity.
-  Qed.
-
-(** [] *)
-
-(** **** Exercise: 2 stars, recommended (beq_natlist) *)
-(** Fill in the definition of [beq_natlist], which compares
-    lists of numbers for equality.  Prove that [beq_natlist l l]
-    yields [true] for every list [l]. *)
-
-Fixpoint beq_natlist (l1 l2 : natlist) : bool :=
-   match l1, l2 with
-    | nil, nil => true
-    | a :: s1', b :: s2' => match beq_nat a b with
-                              | true => beq_natlist s1' s2'
-                              | false => false
-                            end
-    | nil, _ => false
-    | _, nil => false
-   end.
-
-                  
-
-Example test_beq_natlist1 :   (beq_natlist nil nil = true).
-Proof. reflexivity. Qed.
-
-Example test_beq_natlist2 :   beq_natlist [1,2,3] [1,2,3] = true.
-Proof. reflexivity. Qed.
-Example test_beq_natlist3 :   beq_natlist [1,2,3] [1,2,4] = false.
-Proof. reflexivity. Qed.
-
-Check beq_nat_refl.
-
-Theorem beq_natlist_refl : forall l:natlist,
-  true = beq_natlist l l.
-Proof.
-  intros. induction l as [| l'].
-  Case "[]".
-  reflexivity.
-  Case "not []".
-  simpl.
-  rewrite <- beq_nat_refl.
-  rewrite <- IHl.
-  reflexivity.
-  Qed.
-  
-  
-
-
+  (* FILL IN HERE *) Admitted.
 (** [] *)
 
 (* ###################################################### *)
-(** * Extended Exercise: Dictionaries *)
+(** * Dictionaries *)
 
 (** As a final illustration of how fundamental data structures
     can be defined in Coq, here is the declaration of a simple
@@ -1109,35 +981,36 @@ Definition insert (key value : nat) (d : dictionary) : dictionary :=
 Fixpoint find (key : nat) (d : dictionary) : natoption := 
   match d with 
   | empty         => None
-  | record k v d' => if (beq_nat key k) then (Some v) else (find key d')
+  | record k v d' => if (beq_nat key k) 
+                       then (Some v) 
+                       else (find key d')
   end.
 
-(** **** Exercise: 1 star (dictionary_invariant1) *)
+
+
+(** **** Exercise: 1 star (dictionary_invariant1)  *)
 (** Complete the following proof. *)
 
-Theorem dictionary_invariant1 : forall (d : dictionary) (k v: nat),
+Theorem dictionary_invariant1' : forall (d : dictionary) (k v: nat),
   (find k (insert k v d)) = Some v.
 Proof.
-  intros.
-  simpl.
-  rewrite <- beq_nat_refl.
-  reflexivity.
-Qed.
+ (* FILL IN HERE *) Admitted.
+(** [] *)
 
-(** **** Exercise: 1 star (dictionary_invariant2) *)
+(** **** Exercise: 1 star (dictionary_invariant2)  *)
 (** Complete the following proof. *)
 
-Theorem dictionary_invariant2 : forall (d : dictionary) (m n o: nat),
-  (beq_nat m n) = false -> (find m d) = (find m (insert n o d)).
+Theorem dictionary_invariant2' : forall (d : dictionary) (m n o: nat),
+  beq_nat m n = false -> find m d = find m (insert n o d).
 Proof.
-  intros.
-  simpl.
-  rewrite H.
-  reflexivity.
-  Qed.
+ (* FILL IN HERE *) Admitted.
 (** [] *)
+
+
 
 End Dictionary.
 
 End NatList.
+
+(** $Date: 2014-12-31 11:17:56 -0500 (Wed, 31 Dec 2014) $ *)
 
