Types.v
@@ -1,10 +1,10 @@
 (** * Types: Type Systems *)
 
-(* $Date: 2011-06-03 13:58:55 -0400 (Fri, 03 Jun 2011) $ *)
-
 Require Export Smallstep.
 
-(** Our next topic, a large one, is _type systems_ -- static program
+Hint Constructors multi.  
+
+(** Our next major topic is _type systems_ -- static program
     analyses that classify expressions according to the "shapes" of
     their results.  We'll begin with a typed version of a very simple
     language with just booleans and numbers, to introduce the basic
@@ -13,262 +13,6 @@ Require Export Smallstep.
     on to the _simply typed lambda-calculus_, which lives at the core
     of every modern functional programming language (including
     Coq). *)
-
-(* ###################################################################### *)
-(** * More Automation *)
-
-(** Before we start, let's spend a little time learning to use
-    some of Coq's more powerful automation features... *)
-
-(* ###################################################################### *)
-(** ** The [auto] and [eauto] Tactics *)
-
-(** The [auto] tactic solves goals that are solvable by any combination of 
-     - [intros],
-     - [apply] (with a local hypothesis, by default), and
-     - [reflexivity].
-       
-    The [eauto] tactic works just like [auto], except that it uses
-    [eapply] instead of [apply]. *)
-
-(** Using [auto] is always "safe" in the sense that it will never fail
-    and will never change the proof state: either it completely solves
-    the current goal, or it does nothing.
-
-    Here is a contrived example: *)
-
-Lemma auto_example_1 : forall P Q R S T U : Prop,
-  (P -> Q) ->
-  (P -> R) ->
-  (T -> R) ->
-  (S -> T -> U) ->
-  ((P->Q) -> (P->S)) ->
-  T ->
-  P ->
-  U.
-Proof. auto. Qed.
-
-(** When searching for potential proofs of the current goal, [auto]
-    and [eauto] consider the hypotheses in the current context
-    together with a _hint database_ of other lemmas and constructors.
-    Some of the lemmas and constructors we've already seen -- e.g.,
-    [conj], [or_introl], and [or_intror] -- are installed in this hint
-    database by default. *)
-
-Lemma auto_example_2 : forall P Q R : Prop,
-  Q ->
-  (Q -> R) ->
-  P \/ (Q /\ R).
-Proof.
-  auto. Qed.
-
-(** We can extend the hint database just for the purposes of one
-    application of [auto] or [eauto] by writing [auto using ...].
-    E.g., if [conj], [or_introl], and [or_intror] had _not_ already
-    been in the hint database, we could have done this instead: *)
-
-Lemma auto_example_2a : forall P Q R : Prop,
-  Q ->
-  (Q -> R) ->
-  P \/ (Q /\ R).
-Proof.
-  auto using conj, or_introl, or_intror.  Qed.
-
-(** Of course, in any given development there will also be some of our
-    own specific constructors and lemmas that are used very often in
-    proofs.  We can add these to the global hint database by writing
-      Hint Resolve T.
-    at the top level, where [T] is a top-level theorem or a
-    constructor of an inductively defined proposition (i.e., anything
-    whose type is an implication).  As a shorthand, we can write
-      Hint Constructors c.
-    to tell Coq to do a [Hint Resolve] for _all_ of the constructors
-    from the inductive definition of [c].
-
-    It is also sometimes necessary to add
-      Hint Unfold d.
-    where [d] is a defined symbol, so that [auto] knows to expand
-    uses of [d] and enable further possibilities for applying
-    lemmas that it knows about. *)
-
-(** Here are some [Hint]s we will find useful. *)
-
-Hint Constructors multi.
-Hint Resolve beq_id_eq beq_id_false_not_eq.
-
-(** Warning: Just as with Coq's other automation facilities, it is
-    easy to overuse [auto] and [eauto] and wind up with proofs that
-    are impossible to understand later! 
-
-    Also, overuse of [eauto] can make proof scripts very slow.  Get in
-    the habit of using [auto] most of the time and [eauto] only when
-    necessary. 
-
-    For much more detailed information about using [auto] and [eauto],
-    see the chapter [UseAuto]. *)
-
-(* ###################################################################### *)
-(** ** The [Proof with] Tactic *)
-
-(** If you start a proof by saying [Proof with (tactic)] instead of
-    just [Proof], then writing [...] instead of [.] after a tactic in
-    the body of the proof will try to solve all generated subgoals
-    with [tactic] (and fail if this doesn't work).
-
-    One common use of this facility is "[Proof with auto]" (or
-    [eauto]).  We'll see many examples of this later in the file. *)
-
-(* ###################################################################### *)
-(** ** The [solve by inversion] Tactic *)
-
-(** Here's another nice automation feature: it often arises that the
-    context contains a contradictory assumption and we want to use
-    [inversion] on it to solve the goal.  We'd like to be able to say
-    to Coq, "find a contradictory assumption and invert it" without
-    giving its name explicitly.
-
-    Doing [solve by inversion] will find a hypothesis that can be
-    inverted to solve the goal, if there is one.  The tactics [solve
-    by inversion 2] and [solve by inversion 3] are slightly fancier
-    versions which will perform two or three inversions in a row, if
-    necessary, to solve the goal. 
-    
-    (These tactics are not actually built into Coq -- their
-    definitions are in [Sflib].) 
-
-    Caution: Overuse of [solve by inversion] can lead to slow proof
-    scripts. *)
-
-(* ###################################################################### *)
-(** ** The [try solve] Tactic *)
-
-(** If [t] is a tactic, then [try solve [t]] is a tactic that
-      - if [t] solves the goal, behaves just like [t], or
-      - if [t] cannot completely solve the goal, does
-        nothing.
-
-    More generally, [try solve [t1 | t2 | ...]] will try to solve the
-    goal by using [t1], [t2], etc.  If none of them succeeds in
-    completely solving the goal, then [try solve [t1 | t2 | ...]] does
-    nothing. *)
-
-(* ###################################################################### *)
-(** ** The [f_equal] Tactic *)
-
-(** [f_equal] replaces a goal of the form [f x1 x2 ... xn = f y1 y2
-    ... yn], where [f] is some function, with the subgoals [x1 = y1],
-    [x2 = y2],...,[xn = yn].  It is useful for avoiding explicit
-    rewriting steps, and often the generated subgoals can be quickly
-    cleared by [auto].  This tactic is not fundamental, in the sense
-    that it can always be replaced by a sequence of [assert]s.
-    However in some cases it can be very handy. *)
-
-(* ###################################################################### *)
-(** ** The [normalize] Tactic *)
-
-(** When experimenting with definitions of programming languages in
-    Coq, we often want to see what a particular concrete term steps
-    to -- i.e., we want to find proofs for goals of the form [t ==>*
-    t'], where [t] is a completely concrete term and [t'] is unknown.
-    These proofs are simple but repetitive to do by hand. Consider for
-    example reducing an arithmetic expression using the small-step
-    relation [astep] defined in the previous chapter: *)
-
-Definition amultistep st := multi (astep st).
-Notation " t '/' st '==>a*' t' " := (amultistep st t t')
-  (at level 40, st at level 39).
-
-Example astep_example1 : 
-  (APlus (ANum 3) (AMult (ANum 3) (ANum 4))) / empty_state 
-  ==>a* (ANum 15).
-Proof.
-  apply multi_step with (APlus (ANum 3) (ANum 12)).
-    apply AS_Plus2. 
-      apply av_num. 
-      apply AS_Mult.
-  apply multi_step with (ANum 15).
-    apply AS_Plus.
-  apply multi_refl.
-Qed.
-
-(** We repeatedly applied [multi_step] until we got to a normal
-    form. The proofs that the intermediate steps are possible are
-    simple enough that [auto], with appropriate hints, can solve
-    them. *)
-
-Hint Constructors astep aval.
-Example astep_example1' : 
-  (APlus (ANum 3) (AMult (ANum 3) (ANum 4))) / empty_state 
-  ==>a* (ANum 15).
-Proof.
-  eapply multi_step. auto. simpl.
-  eapply multi_step. auto. simpl.
-  apply multi_refl.
-Qed.
-
-(** The following custom [Tactic Notation] definition captures this
-    pattern.  In addition, before each [multi_step] we print out the
-    current goal, so that the user can follow how the term is being
-    evaluated. *)
-
-Tactic Notation "print_goal" := match goal with |- ?x => idtac x end.
-Tactic Notation "normalize" := 
-   repeat (print_goal; eapply multi_step ; 
-             [ (eauto 10; fail) | (instantiate; simpl)]);
-   apply multi_refl.
-
-Example astep_example1'' : 
-  (APlus (ANum 3) (AMult (ANum 3) (ANum 4))) / empty_state 
-  ==>a* (ANum 15).
-Proof.
-  normalize.
-  (* At this point in the proof script, the Coq response shows 
-     a trace of how the expression evaluated. 
-
-   (APlus (ANum 3) (AMult (ANum 3) (ANum 4)) / empty_state ==>a* ANum 15)
-   (multi (astep empty_state) (APlus (ANum 3) (ANum 12)) (ANum 15))
-   (multi (astep empty_state) (ANum 15) (ANum 15))
-*)
-Qed.
-
-(** The [normalize] tactic also provides a simple way to calculate
-    what the normal form of a term is, by proving a goal with an
-    existential variable in it. *)
-
-Example astep_example1''' : exists e',
-  (APlus (ANum 3) (AMult (ANum 3) (ANum 4))) / empty_state 
-  ==>a* e'.
-Proof.
-  eapply ex_intro. normalize.
-(* This time the trace will be:
-
-    (APlus (ANum 3) (AMult (ANum 3) (ANum 4)) / empty_state ==>a* ??)
-    (multi (astep empty_state) (APlus (ANum 3) (ANum 12)) ??)
-    (multi (astep empty_state) (ANum 15) ??)
-
-   where ?? is the variable ``guessed'' by eapply.
-*)
-Qed.
-
-
-(** **** Exercise: 1 star (normalize_ex) *)
-Theorem normalize_ex : exists e',
-  (AMult (ANum 3) (AMult (ANum 2) (ANum 1))) / empty_state 
-  ==>a* e'.
-Proof.
-  (* FILL IN HERE *) Admitted.
-
-(** [] *)
-
-(** **** Exercise: 1 star, optional (normalize_ex') *)
-(** This time prove it by using [apply] instead of [eapply]. *)
-
-Theorem normalize_ex' : exists e',
-  (AMult (ANum 3) (AMult (ANum 2) (ANum 1))) / empty_state 
-  ==>a* e'.
-Proof.
-  (* FILL IN HERE *) Admitted.
-(** [] *)
 
 (* ###################################################################### *)
 (** * Typed Arithmetic Expressions *)
@@ -282,13 +26,7 @@ Proof.
     but just two kinds (numbers and booleans) already gives us enough
     material to tell an interesting story.
 
-    The language definition is completely routine.  The only thing to
-    notice is that we are _not_ using the [asnum]/[aslist] trick that
-    we used in chapter [HoareList] to make all the operations total by
-    forcibly coercing the arguments to [+] (for example) into numbers.
-    Instead, we simply let terms get stuck if they try to use an
-    operator with the wrong kind of operands: the [step] relation
-    doesn't relate them to anything. *)
+    The language definition is completely routine.  *)
 
 (* ###################################################################### *)
 (** ** Syntax *)
@@ -327,11 +65,13 @@ Definition value (t:tm) := bvalue t \/ nvalue t.
 
 Hint Constructors bvalue nvalue.
 Hint Unfold value.  
+Hint Unfold extend.
 
 (* ###################################################################### *)
 (** ** Operational Semantics *)
 
-(** Informally:
+(** Informally: *)
+(**
                     ------------------------------                  (ST_IfTrue)
                     if true then t1 else t2 ==> t1
 
@@ -368,8 +108,9 @@ Hint Unfold value.
                               t1 ==> t1'
                        ------------------------                     (ST_Iszero)
                        iszero t1 ==> iszero t1'
-    Formally:
 *)
+
+(** Formally: *)
 
 Reserved Notation "t1 '==>' t2" (at level 40).
 
@@ -412,15 +153,16 @@ Tactic Notation "step_cases" tactic(first) ident(c) :=
   | Case_aux c "ST_Iszero" ].
 
 Hint Constructors step.
-
 (** Notice that the [step] relation doesn't care about whether
     expressions make global sense -- it just checks that the operation
     in the _next_ reduction step is being applied to the right kinds
-    of operands.  For example, the term [succ true] (i.e., [tsucc
-    ttrue] in the formal syntax) cannot take a step, but the
-    almost-as-obviously-nonsensical term
+    of operands.  
+
+    For example, the term [succ true] (i.e., [tsucc ttrue] in the
+    formal syntax) cannot take a step, but the almost as obviously
+    nonsensical term
        succ (if true then true else true) 
-    can take _one_ step. *)
+    can take a step (once, before becoming stuck). *)
 
 (* ###################################################################### *)
 (** ** Normal Forms and Values *)
@@ -439,7 +181,7 @@ Definition stuck (t:tm) : Prop :=
 
 Hint Unfold stuck.
 
-(** **** Exercise: 2 stars (some_term_is_stuck) *)
+(** **** Exercise: 2 stars (some_term_is_stuck)  *)
 Example some_term_is_stuck :
   exists t, stuck t.
 Proof.
@@ -451,7 +193,7 @@ Proof.
     important because it shows we did not accidentally define things
     so that some value could still take a step. *)
 
-(** **** Exercise: 3 stars, optional (value_is_nf) *)
+(** **** Exercise: 3 stars, advanced (value_is_nf)  *)
 (** Hint: You will reach a point in this proof where you need to
     use an induction to reason about a term that is known to be a
     numeric value.  This induction can be performed either over the
@@ -466,7 +208,8 @@ Proof.
   (* FILL IN HERE *) Admitted.
 (** [] *)
 
-(** **** Exercise: 3 stars, optional (step_deterministic) *)
+
+(** **** Exercise: 3 stars, optional (step_deterministic)  *)
 (** Using [value_is_nf], we can show that the [step] relation is
     also deterministic... *)
 
@@ -475,6 +218,8 @@ Theorem step_deterministic:
 Proof with eauto.
   (* FILL IN HERE *) Admitted.
 (** [] *)
+
+
 
 (* ###################################################################### *)
 (** ** Typing *)
@@ -491,59 +236,62 @@ Inductive ty : Type :=
   | TNat : ty.
 
 (** In informal notation, the typing relation is often written
-    [|- t : T], pronounced "[t] has type [T]."  The [|-] symbol is
+    [|- t \in T], pronounced "[t] has type [T]."  The [|-] symbol is
     called a "turnstile".  (Below, we're going to see richer typing
     relations where an additional "context" argument is written to the
     left of the turnstile.  Here, the context is always empty.) *)
 (** 
-                            --------------                             (T_True)
-                            |- true : Bool
+                           ----------------                            (T_True)
+                           |- true \in Bool
 
-                           ---------------                            (T_False)
-                           |- false : Bool
+                          -----------------                           (T_False)
+                          |- false \in Bool
 
-                |- t1 : Bool    |- t2 : T    |- t3 : T 
-                --------------------------------------                   (T_If)
-                     |- if t1 then t2 else t3 : T
+             |- t1 \in Bool    |- t2 \in T    |- t3 \in T
+             --------------------------------------------                (T_If)
+                    |- if t1 then t2 else t3 \in T
 
-                              ----------                               (T_Zero)
-                              |- 0 : Nat
+                             ------------                              (T_Zero)
+                             |- 0 \in Nat
                               
-                             |- t1 : Nat
-                           ----------------                            (T_Succ)
-                           |- succ t1 : Nat
+                            |- t1 \in Nat
+                          ------------------                           (T_Succ)
+                          |- succ t1 \in Nat
 
-                             |- t1 : Nat
-                           ----------------                            (T_Pred)
-                           |- pred t1 : Nat
+                            |- t1 \in Nat
+                          ------------------                           (T_Pred)
+                          |- pred t1 \in Nat
 
-                             |- t1 : Nat
-                         -------------------                         (T_IsZero)
-                         |- iszero t1 : Bool
+                            |- t1 \in Nat
+                        ---------------------                        (T_IsZero)
+                        |- iszero t1 \in Bool
 *)
+
+Reserved Notation "'|-' t '\in' T" (at level 40).
 
 Inductive has_type : tm -> ty -> Prop :=
   | T_True : 
-       has_type ttrue TBool
+       |- ttrue \in TBool
   | T_False : 
-       has_type tfalse TBool
+       |- tfalse \in TBool
   | T_If : forall t1 t2 t3 T,
-       has_type t1 TBool ->
-       has_type t2 T ->
-       has_type t3 T ->
-       has_type (tif t1 t2 t3) T
+       |- t1 \in TBool ->
+       |- t2 \in T ->
+       |- t3 \in T ->
+       |- tif t1 t2 t3 \in T
   | T_Zero : 
-       has_type tzero TNat
+       |- tzero \in TNat
   | T_Succ : forall t1,
-       has_type t1 TNat ->
-       has_type (tsucc t1) TNat
+       |- t1 \in TNat ->
+       |- tsucc t1 \in TNat
   | T_Pred : forall t1,
-       has_type t1 TNat ->
-       has_type (tpred t1) TNat
+       |- t1 \in TNat ->
+       |- tpred t1 \in TNat
   | T_Iszero : forall t1,
-       has_type t1 TNat ->
-       has_type (tiszero t1) TBool.
+       |- t1 \in TNat ->
+       |- tiszero t1 \in TBool
 
+where "'|-' t '\in' T" := (has_type t T).
 
 Tactic Notation "has_type_cases" tactic(first) ident(c) :=
   first;
@@ -561,7 +309,7 @@ Hint Constructors has_type.
     the type of the normal form of a term. *)
 
 Example has_type_1 : 
-  has_type (tif tfalse tzero (tsucc tzero)) TNat.
+  |- tif tfalse tzero (tsucc tzero) \in TNat.
 Proof. 
   apply T_If. 
     apply T_False.
@@ -575,17 +323,43 @@ Qed.
     proof automatically.) *)
 
 Example has_type_not : 
-  ~ has_type (tif tfalse tzero ttrue) TBool.
+  ~ (|- tif tfalse tzero ttrue \in TBool).
 Proof.
   intros Contra. solve by inversion 2.  Qed.
 
-(** **** Exercise: 1 star (succ_hastype_nat__hastype_nat) *)
+(** **** Exercise: 1 star, optional (succ_hastype_nat__hastype_nat)  *)
 Example succ_hastype_nat__hastype_nat : forall t,
-  has_type (tsucc t) TNat ->
-  has_type t TNat.  
+  |- tsucc t \in TNat ->
+  |- t \in TNat.  
 Proof.
   (* FILL IN HERE *) Admitted.
 (** [] *)
+
+(* ###################################################################### *)
+(** ** Canonical forms *)
+
+(** The following two lemmas capture the basic property that defines
+    the shape of well-typed values.  They say that the definition of value
+    and the typing relation agree. *)
+
+Lemma bool_canonical : forall t,
+  |- t \in TBool -> value t -> bvalue t.
+Proof.
+  intros t HT HV.
+  inversion HV; auto.
+
+  induction H; inversion HT; auto.
+Qed.
+
+Lemma nat_canonical : forall t,
+  |- t \in TNat -> value t -> nvalue t.
+Proof.
+  intros t HT HV.
+  inversion HV.
+  inversion H; subst; inversion HT.   
+
+  auto.  
+Qed.
 
 (* ###################################################################### *)
 (** ** Progress *)
@@ -593,23 +367,48 @@ Proof.
 (** The typing relation enjoys two critical properties.  The first is
     that well-typed normal forms are values (i.e., not stuck). *)
 
-(** **** Exercise: 3 stars, recommended (finish_progress_informal) *)
-(** Complete the following proof: *)
+Theorem progress : forall t T,
+  |- t \in T ->
+  value t \/ exists t', t ==> t'.
 
-(** _Theorem_: If [|- t : T], then either [t] is a value or else 
+(** **** Exercise: 3 stars (finish_progress)  *)
+(** Complete the formal proof of the [progress] property.  (Make sure
+    you understand the informal proof fragment in the following
+    exercise before starting -- this will save you a lot of time.) *)
+
+Proof with auto.
+  intros t T HT.
+  has_type_cases (induction HT) Case...
+  (* The cases that were obviously values, like T_True and
+     T_False, were eliminated immediately by auto *)
+  Case "T_If".
+    right. inversion IHHT1; clear IHHT1.
+    SCase "t1 is a value".
+    apply (bool_canonical t1 HT1) in H.
+    inversion H; subst; clear H.
+      exists t2...
+      exists t3...
+    SCase "t1 can take a step".
+      inversion H as [t1' H1].
+      exists (tif t1' t2 t3)...
+  (* FILL IN HERE *) Admitted.
+(** [] *)
+
+(** **** Exercise: 3 stars, advanced (finish_progress_informal)  *)
+(** Complete the corresponding informal proof: *)
+
+(** _Theorem_: If [|- t \in T], then either [t] is a value or else 
     [t ==> t'] for some [t']. *)
 
-(** _Proof_: By induction on a derivation of [|- t : T].
+(** _Proof_: By induction on a derivation of [|- t \in T].
 
       - If the last rule in the derivation is [T_If], then [t = if t1
-        then t2 else t3], with [|- t1 : Bool], [|- t2 : T] and [|- t3
-        : T].  By the IH, either [t1] is a value or else [t1] can step
+        then t2 else t3], with [|- t1 \in Bool], [|- t2 \in T] and [|- t3
+        \in T].  By the IH, either [t1] is a value or else [t1] can step
         to some [t1'].  
 
-            - If [t1] is a value, then it is either an [nvalue] or a
-              [bvalue].  But it cannot be an [nvalue], because we know
-              [|- t1 : Bool] and there are no rules assigning type
-              [Bool] to any term that could be an [nvalue].  So [t1]
+            - If [t1] is a value, then by the canonical forms lemmas
+              and the fact that [|- t1 \in Bool] we have that [t1] 
               is a [bvalue] -- i.e., it is either [true] or [false].
               If [t1 = true], then [t] steps to [t2] by [ST_IfTrue],
               while if [t1 = false], then [t] steps to [t3] by
@@ -620,40 +419,14 @@ Proof.
               [t].
 
     (* FILL IN HERE *)
-[]
-*)
-
-(** **** Exercise: 3 stars (finish_progress) *)
-Theorem progress : forall t T,
-  has_type t T ->
-  value t \/ exists t', t ==> t'.
-Proof with auto.
-  intros t T HT.
-  has_type_cases (induction HT) Case...
-  (* The cases that were obviously values, like T_True and
-     T_False, were eliminated immediately by auto *)
-  Case "T_If".
-    right. inversion IHHT1; clear IHHT1.
-    SCase "t1 is a value". inversion H; clear H.
-      SSCase "t1 is a bvalue". inversion H0; clear H0.
-        SSSCase "t1 is ttrue".
-          exists t2...
-        SSSCase "t1 is tfalse". 
-          exists t3...
-      SSCase "t1 is an nvalue".
-        solve by inversion 2.  (* on H and HT1 *)
-    SCase "t1 can take a step".
-      inversion H as [t1' H1].
-      exists (tif t1' t2 t3)...
-  (* FILL IN HERE *) Admitted.
-(** [] *)
+[] *)
 
 (** This is more interesting than the strong progress theorem that we
     saw in the Smallstep chapter, where _all_ normal forms were
     values.  Here, a term can be stuck, but only if it is ill
     typed. *)
 
-(** **** Exercise: 1 star (step_review) *)
+(** **** Exercise: 1 star (step_review)  *)
 (** Quick review.  Answer _true_ or _false_.  In this language...
       - Every well-typed normal form is a value.
 
@@ -679,42 +452,16 @@ Proof with auto.
     typing statements as sentences, where the term is the subject and
     the type is the predicate. *)
 
-(** **** Exercise: 3 stars, recommended (finish_preservation_informal) *)
-(** Complete the following proof: *)
-
-(** _Theorem_: If [|- t : T] and [t ==> t'], then [|- t' : T]. *)
-
-(** _Proof_: By induction on a derivation of [|- t : T].
-
-      - If the last rule in the derivation is [T_If], then [t = if t1
-        then t2 else t3], with [|- t1 : Bool], [|- t2 : T] and [|- t3
-        : T].  
-
-        Inspecting the rules for the small-step reduction relation and
-        remembering that [t] has the form [if ...], we see that the
-        only ones that could have been used to prove [t ==> t'] are
-        [ST_IfTrue], [ST_IfFalse], or [ST_If].
-
-           - If the last rule was [ST_IfTrue], then [t' = t2].  But we
-             know that [|- t2 : T], so we are done.
-
-           - If the last rule was [ST_IfFalse], then [t' = t3].  But we
-             know that [|- t3 : T], so we are done.
-
-           - If the last rule was [ST_If], then [t' = if t1' then t2
-             else t3], where [t1 ==> t1'].  We know [|- t1 : Bool] so,
-             by the IH, [|- t1' : Bool].  The [T_If] rule then gives us
-             [|- if t1' then t2 else t3 : T], as required.
-
-    (* FILL IN HERE *)
-[]
-*)
-
-(** **** Exercise: 2 stars (finish_preservation) *)
 Theorem preservation : forall t t' T,
-  has_type t T ->
+  |- t \in T ->
   t ==> t' ->
-  has_type t' T.
+  |- t' \in T.
+
+(** **** Exercise: 2 stars (finish_preservation)  *)
+(** Complete the formal proof of the [preservation] property.  (Again,
+    make sure you understand the informal proof fragment in the
+    following exercise first.) *)
+
 Proof with auto.
   intros t t' T HT HE.
   generalize dependent t'.
@@ -724,7 +471,7 @@ Proof with auto.
          (* and we can deal with several impossible
             cases all at once *)
          try (solve by inversion).
-    Case "T_If". inversion HE; subst.
+    Case "T_If". inversion HE; subst; clear HE.
       SCase "ST_IFTrue". assumption.
       SCase "ST_IfFalse". assumption.
       SCase "ST_If". apply T_If; try assumption.
@@ -732,7 +479,37 @@ Proof with auto.
     (* FILL IN HERE *) Admitted.
 (** [] *)
 
-(** **** Exercise: 3 stars (preservation_alternate_proof) *)
+(** **** Exercise: 3 stars, advanced (finish_preservation_informal)  *)
+(** Complete the following proof: *)
+
+(** _Theorem_: If [|- t \in T] and [t ==> t'], then [|- t' \in T]. *)
+
+(** _Proof_: By induction on a derivation of [|- t \in T].
+
+      - If the last rule in the derivation is [T_If], then [t = if t1
+        then t2 else t3], with [|- t1 \in Bool], [|- t2 \in T] and [|- t3
+        \in T].  
+
+        Inspecting the rules for the small-step reduction relation and
+        remembering that [t] has the form [if ...], we see that the
+        only ones that could have been used to prove [t ==> t'] are
+        [ST_IfTrue], [ST_IfFalse], or [ST_If].
+
+           - If the last rule was [ST_IfTrue], then [t' = t2].  But we
+             know that [|- t2 \in T], so we are done.
+
+           - If the last rule was [ST_IfFalse], then [t' = t3].  But we
+             know that [|- t3 \in T], so we are done.
+
+           - If the last rule was [ST_If], then [t' = if t1' then t2
+             else t3], where [t1 ==> t1'].  We know [|- t1 \in Bool] so,
+             by the IH, [|- t1' \in Bool].  The [T_If] rule then gives us
+             [|- if t1' then t2 else t3 \in T], as required.
+
+    (* FILL IN HERE *)
+[] *)
+
+(** **** Exercise: 3 stars (preservation_alternate_proof)  *)
 (** Now prove the same property again by induction on the
     _evaluation_ derivation instead of on the typing derivation.
     Begin by carefully reading and thinking about the first few
@@ -741,9 +518,9 @@ Proof with auto.
     not exactly the same. *)
 
 Theorem preservation' : forall t t' T,
-  has_type t T ->
+  |- t \in T ->
   t ==> t' ->
-  has_type t' T.
+  |- t' \in T.
 Proof with eauto.
   (* FILL IN HERE *) Admitted.
 (** [] *)
@@ -758,7 +535,7 @@ Definition multistep := (multi step).
 Notation "t1 '==>*' t2" := (multistep t1 t2) (at level 40).
 
 Corollary soundness : forall t t' T,
-  has_type t T -> 
+  |- t \in T -> 
   t ==>* t' ->
   ~(stuck t').
 Proof. 
@@ -767,30 +544,144 @@ Proof.
   apply IHP.  apply (preservation x y T HT H).
   unfold stuck. split; auto.   Qed.
 
+
+(* ###################################################################### *)
+(** * Aside: the [normalize] Tactic *)
+
+(** When experimenting with definitions of programming languages in
+    Coq, we often want to see what a particular concrete term steps
+    to -- i.e., we want to find proofs for goals of the form [t ==>*
+    t'], where [t] is a completely concrete term and [t'] is unknown.
+    These proofs are simple but repetitive to do by hand. Consider for
+    example reducing an arithmetic expression using the small-step
+    relation [astep]. *)
+
+
+Definition amultistep st := multi (astep st). 
+Notation " t '/' st '==>a*' t' " := (amultistep st t t')
+  (at level 40, st at level 39).
+
+Example astep_example1 : 
+  (APlus (ANum 3) (AMult (ANum 3) (ANum 4))) / empty_state 
+  ==>a* (ANum 15).
+Proof.
+  apply multi_step with (APlus (ANum 3) (ANum 12)).
+    apply AS_Plus2. 
+      apply av_num. 
+      apply AS_Mult.
+  apply multi_step with (ANum 15).
+    apply AS_Plus.
+  apply multi_refl.
+Qed.
+
+(** We repeatedly apply [multi_step] until we get to a normal
+    form. The proofs that the intermediate steps are possible are
+    simple enough that [auto], with appropriate hints, can solve
+    them. *)
+
+Hint Constructors astep aval.
+Example astep_example1' : 
+  (APlus (ANum 3) (AMult (ANum 3) (ANum 4))) / empty_state 
+  ==>a* (ANum 15).
+Proof.
+  eapply multi_step. auto. simpl.
+  eapply multi_step. auto. simpl.
+  apply multi_refl.
+Qed.
+
+
+(** The following custom [Tactic Notation] definition captures this
+    pattern.  In addition, before each [multi_step] we print out the
+    current goal, so that the user can follow how the term is being
+    evaluated. *)
+
+Tactic Notation "print_goal" := match goal with |- ?x => idtac x end.
+Tactic Notation "normalize" := 
+   repeat (print_goal; eapply multi_step ; 
+             [ (eauto 10; fail) | (instantiate; simpl)]);
+   apply multi_refl.
+
+
+Example astep_example1'' : 
+  (APlus (ANum 3) (AMult (ANum 3) (ANum 4))) / empty_state 
+  ==>a* (ANum 15).
+Proof.
+  normalize.
+  (* At this point in the proof script, the Coq response shows 
+     a trace of how the expression evaluated. 
+
+   (APlus (ANum 3) (AMult (ANum 3) (ANum 4)) / empty_state ==>a* ANum 15)
+   (multi (astep empty_state) (APlus (ANum 3) (ANum 12)) (ANum 15))
+   (multi (astep empty_state) (ANum 15) (ANum 15))
+*)
+Qed.
+
+
+(** The [normalize] tactic also provides a simple way to calculate
+    what the normal form of a term is, by proving a goal with an
+    existential variable in it. *)
+
+Example astep_example1''' : exists e',
+  (APlus (ANum 3) (AMult (ANum 3) (ANum 4))) / empty_state 
+  ==>a* e'.
+Proof.
+  eapply ex_intro. normalize.
+
+(* This time, the trace will be:
+
+    (APlus (ANum 3) (AMult (ANum 3) (ANum 4)) / empty_state ==>a* ??)
+    (multi (astep empty_state) (APlus (ANum 3) (ANum 12)) ??)
+    (multi (astep empty_state) (ANum 15) ??)
+
+   where ?? is the variable ``guessed'' by eapply.
+*)
+Qed.
+
+
+(** **** Exercise: 1 star (normalize_ex)  *)
+Theorem normalize_ex : exists e',
+  (AMult (ANum 3) (AMult (ANum 2) (ANum 1))) / empty_state 
+  ==>a* e'.
+Proof.
+  (* FILL IN HERE *) Admitted.
+
+(** [] *)
+
+(** **** Exercise: 1 star, optional (normalize_ex')  *)
+(** For comparison, prove it using [apply] instead of [eapply]. *)
+
+Theorem normalize_ex' : exists e',
+  (AMult (ANum 3) (AMult (ANum 2) (ANum 1))) / empty_state 
+  ==>a* e'.
+Proof.
+  (* FILL IN HERE *) Admitted.
+(** [] *)
+
+
 (* ###################################################################### *)
 (** ** Additional Exercises *)
 
-(** **** Exercise: 2 stars, recommended (subject_expansion) *)
+(** **** Exercise: 2 stars (subject_expansion)  *)
 (** Having seen the subject reduction property, it is reasonable to
     wonder whether the opposity property -- subject _expansion_ --
     also holds.  That is, is it always the case that, if [t ==> t']
-    and [has_type t' T], then [has_type t T]?  If so, prove it.  If
+    and [|- t' \in T], then [|- t \in T]?  If so, prove it.  If
     not, give a counter-example.  (You do not need to prove your
     counter-example in Coq, but feel free to do so if you like.)
 
     (* FILL IN HERE *)
-[]
-*)
+[] *)
 
-(** **** Exercise: 2 stars (variation1) *)
-(** Suppose we add the following two new rules to the reduction
-    relation:
-      | ST_PredTrue : 
-           (tpred ttrue) ==> (tpred tfalse)
-      | ST_PredFalse : 
-           (tpred tfalse) ==> (tpred ttrue)
-   Which of the following properties remain true in the presence
-   of these rules?  For each one, write either "remains true" or
+
+
+
+(** **** Exercise: 2 stars (variation1)  *)
+(** Suppose, that we add this new rule to the typing relation: 
+      | T_SuccBool : forall t,
+           |- t \in TBool ->
+           |- tsucc t \in TBool
+   Which of the following properties remain true in the presence of
+   this rule?  For each one, write either "remains true" or
    else "becomes false." If a property becomes false, give a
    counterexample.
       - Determinism of [step]
@@ -799,52 +690,18 @@ Proof.
 
       - Preservation
 
-[]
-*)
+[] *)
 
-(** **** Exercise: 2 stars (variation2) *)
-(** Suppose, instead, that we add this new rule to the typing relation: 
-      | T_IfFunny : forall t2 t3,
-           has_type t2 TNat ->
-           has_type (tif ttrue t2 t3) TNat
-   Which of the following properties remain true in the presence of
-   this rule?  (Answer in the same style as above.)
-      - Determinism of [step]
-
-      - Progress
-
-      - Preservation
-
-[]
-*)
-
-(** **** Exercise: 2 stars (variation3) *)
-(** Suppose, instead, that we add this new rule to the typing relation: 
-      | T_SuccBool : forall t,
-           has_type t TBool ->
-           has_type (tsucc t) TBool
-   Which of the following properties remain true in the presence of
-   this rule?  (Answer in the same style as above.)
-      - Determinism of [step]
-
-      - Progress
-
-      - Preservation
-
-[]
-*)
-
-(** **** Exercise: 2 stars (variation4) *)
+(** **** Exercise: 2 stars (variation2)  *)
 (** Suppose, instead, that we add this new rule to the [step] relation: 
       | ST_Funny1 : forall t2 t3,
            (tif ttrue t2 t3) ==> t3
    Which of the above properties become false in the presence of
    this rule?  For each one that does, give a counter-example.
 
-[]
-*)
+[] *)
 
-(** **** Exercise: 2 stars (variation5) *)
+(** **** Exercise: 2 stars, optional (variation3)  *)
 (** Suppose instead that we add this rule:
       | ST_Funny2 : forall t1 t2 t2' t3,
            t2 ==> t2' ->
@@ -852,52 +709,47 @@ Proof.
    Which of the above properties become false in the presence of
    this rule?  For each one that does, give a counter-example.
 
-[]
-*)
+[] *)
 
-(** **** Exercise: 2 stars (variation6) *)
+(** **** Exercise: 2 stars, optional (variation4)  *)
 (** Suppose instead that we add this rule:
       | ST_Funny3 : 
           (tpred tfalse) ==> (tpred (tpred tfalse))
    Which of the above properties become false in the presence of
    this rule?  For each one that does, give a counter-example.
 
-[]
-*)
+[] *)
 
-(** **** Exercise: 2 stars (variation7) *)
+(** **** Exercise: 2 stars, optional (variation5)  *)
 (** Suppose instead that we add this rule:
    
       | T_Funny4 : 
-            has_type tzero TBool
+            |- tzero \in TBool
    ]]
    Which of the above properties become false in the presence of
    this rule?  For each one that does, give a counter-example.
 
-[]
-*)
+[] *)
 
-(** **** Exercise: 2 stars (variation8) *)
+(** **** Exercise: 2 stars, optional (variation6)  *)
 (** Suppose instead that we add this rule:
    
       | T_Funny5 : 
-            has_type (tpred tzero) TBool
+            |- tpred tzero \in TBool
    ]]
    Which of the above properties become false in the presence of
    this rule?  For each one that does, give a counter-example.
 
-[]
-*)
+[] *)
 
-(** **** Exercise: 3 stars, optional (more_variations) *)
+(** **** Exercise: 3 stars, optional (more_variations)  *)
 (** Make up some exercises of your own along the same lines as
     the ones above.  Try to find ways of selectively breaking
     properties -- i.e., ways of changing the definitions that
     break just one of the properties and leave the others alone.
-    [] 
-*)
+[] *)
 
-(** **** Exercise: 1 star (remove_predzero) *)
+(** **** Exercise: 1 star (remove_predzero)  *)
 (** The evaluation rule [E_PredZero] is a bit counter-intuitive: we
     might feel that it makes more sense for the predecessor of zero to
     be undefined, rather than being defined to be zero.  Can we
@@ -907,12 +759,12 @@ Proof.
 (* FILL IN HERE *)
 [] *)
 
-(** **** Exercise: 4 stars, optional (prog_pres_bigstep) *)
+(** **** Exercise: 4 stars, advanced (prog_pres_bigstep)  *)
 (** Suppose our evaluation relation is defined in the big-step style.
     What are the appropriate analogs of the progress and preservation
     properties?
 
 (* FILL IN HERE *)
-[]
-*)
+[] *)
 
+(** $Date: 2014-12-31 11:17:56 -0500 (Wed, 31 Dec 2014) $ *)
